Define type subsumption decision algorithm

theories/Extraction/TypeCheck.v
@@ -4,68 +4,103 @@ From Mcltt.Extraction Require Import NbE.
 From Equations Require Import Equations.
 Import Domain_Notations.
 
-Definition nf_subsumption_dec A A' :
-    {nf_subsumption A A'} + {~ nf_subsumption A A'}.
-Proof.
-  destruct A as [i| | | | | |] eqn:HA.
-  1: destruct A' as [j| | | | | |];
-    [destruct (Compare_dec.le_lt_dec i j)| | | | | |];
-    try (right; intro H; dependent destruction H; subst; lia).
-  1: left; mauto 2.
-  all: destruct (nf_eq_dec A A'); subst; mauto;
-    right; intro H; dependent destruction H; congruence.
-Defined.
-
-#[local]
-Ltac impl_obl_tac :=
-  match goal with
-  | |- nbe_order ?G ?M ?A =>
-      (on_all_hyp: fun H => apply soundness in H);
-      destruct_conjs;
-      eapply nbe_order_sound; eassumption
-  | |- False =>
-      (on_all_hyp: fun H => apply completeness in H);
-      destruct_conjs;
-      functional_nbe_rewrite_clear;
-      congruence
-  | _ =>
-      (on_all_hyp: fun H => apply soundness in H);
-      destruct_conjs;
-      functional_nbe_rewrite_clear;
-      mauto
-  end.
-
-#[tactic="impl_obl_tac"]
-Equations conversion_dec G A M (HM : {{ G ⊢ M : A }}) M' (HM' : {{ G ⊢ M' : A }}) : { {{ G ⊢ M ≈ M' : A }} } + { ~ {{ G ⊢ M ≈ M' : A }} } :=
-| G, A, M, HM, M', HM' =>
-    let (W, HW) := nbe_impl G M A _ in
-    let (W', HW') := nbe_impl G M' A _ in
-    match nf_eq_dec W W' with
-    | left _ => left _
-    | right _ => right _
+Section nf_subsumption_dec.
+  #[local]
+  Ltac impl_obl_tac :=
+    match goal with
+    | |- nf_subsumption _ _ => mauto 2
+    | A := _ : nf |- ~ (nf_subsumption _ _) =>
+        let H := fresh "H" in
+        subst A; intro H; dependent destruction H; congruence
+    | |- ~ (nf_subsumption _ _) =>
+        let H := fresh "H" in
+        intro H; dependent destruction H; lia
     end.
-Next Obligation. impl_obl_tac. Qed.
 
-Equations? typ_subsumption_dec G i A (HA : {{ G ⊢ A : Type@i }}) A' (HA' : {{ G ⊢ A' : Type@i }}) : { {{ G ⊢ A ⊆ A' }} } + { ~ {{ G ⊢ A ⊆ A' }} } :=
-| G, i, A, HA, A', HA' =>
-    let (W, HW) := nbe_impl G A {{{ Type@i }}} _ in
-    let (W', HW') := nbe_impl G A' {{{ Type@i }}} _ in
-    match nf_subsumption_dec W W' with
-    | left _ => left _
-    | right _ => right _
+  #[tactic=impl_obl_tac]
+  Equations nf_subsumption_dec A A' : {nf_subsumption A A'} + {~ nf_subsumption A A'} :=
+  | n{{{ Type@i }}}, n{{{ Type@j }}} =>
+      match Compare_dec.le_lt_dec i j with
+      | left _ => left _
+      | right _ => right _
+      end
+  (* Here we have a separate clause for n{{{ Type@i }}} so that we can extract a more efficient code *)
+  | n{{{ Type@i }}}, _ => right _
+  | A, A' =>
+      match nf_eq_dec A A' with
+      | left _ => left _
+      | right _ => right _
+      end.
+End nf_subsumption_dec.
+
+Section conversion_dec.
+  #[local]
+  Ltac impl_obl_tac :=
+    match goal with
+    | |- nbe_order ?G ?M ?A =>
+        (on_all_hyp: fun H => apply soundness in H);
+        destruct_conjs;
+        eapply nbe_order_sound; eassumption
+    | |- False =>
+        (on_all_hyp: fun H => apply completeness in H);
+        destruct_conjs;
+        functional_nbe_rewrite_clear;
+        congruence
+    | _ =>
+        (on_all_hyp: fun H => apply soundness in H);
+        destruct_conjs;
+        functional_nbe_rewrite_clear;
+        mauto
     end.
-Proof.
-  - impl_obl_tac.
-  - impl_obl_tac.
-  - (on_all_hyp: fun H => apply soundness in H).
-    destruct_conjs.
-    functional_nbe_rewrite_clear.
-    rename HA into W.
-    rename HA' into W'.
-    assert {{ G ⊢ W : Type@i }} by (gen_presups; eassumption).
-    assert {{ G ⊢ W' : Type@i }} by (gen_presups; eassumption).
-    assert {{ G ⊢ W ⊆ W' }} by mauto.
-    etransitivity; mauto.
-  - admit.
-Abort.
-  
+
+  #[tactic="impl_obl_tac"]
+  Equations? conversion_dec G A M (HM : {{ G ⊢ M : A }}) M' (HM' : {{ G ⊢ M' : A }}) : { {{ G ⊢ M ≈ M' : A }} } + { ~ {{ G ⊢ M ≈ M' : A }} } :=
+  | G, A, M, HM, M', HM' =>
+      let (W, HW) := nbe_impl G M A _ in
+      let (W', HW') := nbe_impl G M' A _ in
+      match nf_eq_dec W W' with
+      | left _ => left _
+      | right _ => right _
+      end.
+  Proof.
+    intro. impl_obl_tac.
+  Qed.
+End conversion_dec.
+
+Section typ_subsumption_dec.
+  #[local]
+  Ltac impl_obl_tac :=
+    match goal with
+    | |- nbe_order ?G ?M ?A =>
+        (on_all_hyp: fun H => apply soundness in H);
+        destruct_conjs;
+        eapply nbe_order_sound; eassumption
+    | H: nbe ?G ?A {{{ Type@?i }}} ?W, H': nbe ?G ?A' {{{ Type@?i' }}} ?W' |- {{ ~?G ⊢ ~?A ⊆ ~?A' }} =>
+        (on_all_hyp: fun H => apply soundness in H);
+        destruct_conjs;
+        functional_nbe_rewrite_clear;
+        rename HA into W;
+        rename HA' into W';
+        assert {{ G ⊢ W : Type@i }} by (gen_presups; eassumption);
+        assert {{ G ⊢ W' : Type@i }} by (gen_presups; eassumption);
+        assert {{ G ⊢ W ⊆ W' }} by mauto;
+        etransitivity;
+        mauto
+    | H: ~ (nf_subsumption ?W ?W') |- ~ {{ ~?G ⊢ ~?A ⊆ ~?A' }} =>
+        contradict H;
+        apply completeness_for_typ_subsumption in H;
+        destruct_conjs;
+        functional_nbe_rewrite_clear;
+        eassumption
+    end.
+
+  #[tactic="impl_obl_tac"]
+  Equations typ_subsumption_dec G i A (HA : {{ G ⊢ A : Type@i }}) A' (HA' : {{ G ⊢ A' : Type@i }}) : { {{ G ⊢ A ⊆ A' }} } + { ~ {{ G ⊢ A ⊆ A' }} } :=
+  | G, i, A, HA, A', HA' =>
+      let (W, HW) := nbe_impl G A {{{ Type@i }}} _ in
+      let (W', HW') := nbe_impl G A' {{{ Type@i }}} _ in
+      match nf_subsumption_dec W W' with
+      | left _ => left _
+      | right _ => right _
+      end.
+End typ_subsumption_dec.
